Add `TermVar`

Stlc/Basic.lean
@@ -1,13 +1,16 @@
 namespace Stlc
 
+def TermVar : Type := String
+deriving DecidableEq
+
 inductive Ty : Type
 | bool
 | arrow : Ty → Ty → Ty
 deriving DecidableEq
 
 inductive Term : Type
-| var : String → Term
-| abs : String → Ty → Term → Term
+| var : TermVar → Term
+| abs : TermVar → Ty → Term → Term
 | app : Term → Term → Term
 | bool : Bool → Term
 | ite : Term → Term → Term → Term
